language_formalisation/type_system/declarational.v
@@ -7,7 +7,6 @@ Add LoadPath "C:\Users\Ziga\Documents\Ziga_podatki\PHD\language_formalisation\su
 Require Export syntax syntax_lemmas subtyping substitution.
 
 
-
 Fixpoint handle_tmpl h T :=
   match T with
   | TApp x v => App (Var x) v
@@ -23,17 +22,6 @@ Fixpoint handle_tmpl h T :=
       end
   end.
 
-Fixpoint tctx_len Z :=
-  match Z with
-  | TCtxØ => 0
-  | TCtxU Z _ => S (tctx_len Z)
-  end.
-
-Fixpoint join_ctxs Γ Z D :=
-  match Z with
-  | TCtxØ => Γ
-  | TCtxU Z A => CtxU (join_ctxs Γ Z D) (TyFun A D)
-  end.
 
 (* ========================================================================== *)
 Inductive wf_vtype : vtype -> Prop :=
@@ -112,7 +100,7 @@ with has_vtype' : ctx -> val -> vtype -> Prop :=
     has_vtype' Γ (Fun x c) (TyFun A C)
 | TypeHandler Γ x c_ret h A Σ E D :
     has_ctype (CtxU Γ A) c_ret D ->
-    has_htype Γ h Σ D -> respects h Σ D E ->
+    has_htype Γ h Σ D -> respects Γ h Σ D E ->
     has_vtype' Γ (Handler x c_ret h) (TyHandler (CTy A Σ E) D)
 | TypeVSubtype Γ v A A' :
     has_vtype Γ v A -> vsubtype A A' -> has_vtype' Γ v A'
@@ -174,18 +162,27 @@ with has_htype' : ctx -> hcases -> sig -> ctype -> Prop :=
 
 (* ========================================================================== *)
 
-with respects : hcases -> sig -> ctype -> eqs -> Prop :=
-| RespectEqsØ h Σ D : respects h Σ D EqsØ
-| RespectEqsU h Σ D E Γ Z T1 T2 :
-    respects h Σ D E -> 
-    ceq D (join_ctxs Γ Z D)
-      (handle_tmpl (Sub.h_shift h (tctx_len Z) 0) T1)
-      (handle_tmpl (Sub.h_shift h (tctx_len Z) 0) T2)
-    -> respects h Σ D (EqsU E Γ Z T1 T2)
+with respects : ctx -> hcases -> sig -> ctype -> eqs -> Prop :=
+| Respects Γ h Σ D E :
+    wf_ctx Γ -> wf_sig Σ -> wf_ctype D -> wf_eqs E Σ ->
+    respects' Γ h Σ D E -> respects Γ h Σ D E 
 
-with veq : vtype -> ctx -> val -> val -> Prop :=
-| Veq A Γ v1 v2 : veq A Γ v1 v2 (* Accepts everything! *)
+with respects' : ctx -> hcases -> sig -> ctype -> eqs -> Prop :=
+| RespectEqsØ Γ h Σ D : respects' Γ h Σ D EqsØ
+| RespectEqsU Γ h Σ D E Γ' Z T1 T2 :
+    respects Γ h Σ D E -> 
+    ceq D (join_ctx_tctx (join_ctxs Γ Γ') Z D)
+      (handle_tmpl (Sub.h_shift h (ctx_len Γ' + tctx_len Z) 0) T1)
+      (handle_tmpl (Sub.h_shift h (ctx_len Γ' + tctx_len Z) 0) T2)
+    -> respects' Γ h Σ D (EqsU E Γ' Z T1 T2)
 
-with ceq : ctype -> ctx -> comp -> comp -> Prop :=
-| Ceq C Γ c1 c2 : ceq C Γ c1 c2 (* Accepts everything! *)
+with veq : vtype -> ctx -> val -> val -> Prop := 
+| Veq A Γ v1 v2 : wf_vtype A -> wf_ctx Γ -> veq' A Γ v1 v2 -> veq A Γ v1 v2
+
+with veq': vtype -> ctx -> val -> val -> Prop :=
+
+with ceq : ctype -> ctx -> comp -> comp -> Prop := 
+| Ceq C Γ c1 c2 : wf_ctype C -> wf_ctx Γ -> ceq' C Γ c1 c2 -> ceq C Γ c1 c2
+
+with ceq' : ctype -> ctx -> comp -> comp -> Prop := 
 .
