language_formalisation/type_system/type_aux_lemmas.v
@@ -11,6 +11,40 @@ Require Export substitution_lemmas subtyping subtyping_lemmas wf_lemmas.
 Ltac inv H := inversion H; clear H; subst.
 
 
+Fixpoint v_shift_too_high Γ v A n cut :
+  has_vtype Γ v A -> cut > ctx_len Γ -> Sub.v_shift v n cut = v
+with c_shift_too_high Γ c C n cut :
+  has_ctype Γ c C -> cut > ctx_len Γ -> Sub.c_shift c n cut = c
+with h_shift_too_high Γ h Σ D n cut :
+  has_htype Γ h Σ D -> cut > ctx_len Γ -> Sub.h_shift h n cut = h.
+Proof.
+{
+intros types high. destruct v; simpl; try f_equal.
++ destruct v. eapply shape_var in types. destruct types as [A'[gets]].
+  apply ctx_len_gets in gets. destruct (cut <=? v0) eqn:cmp. 
+  apply leb_complete in cmp. omega. reflexivity.
++ reflexivity.
++ eapply shape_inl_full in types. 2: reflexivity. destruct types as [A'[B']].
+  eapply v_shift_too_high. 2: eauto. destruct H. eauto.
++ eapply shape_inr_full in types. 2: reflexivity. destruct types as [A'[B']].
+  eapply v_shift_too_high. 2: eauto. destruct H. eauto.
+
+
+Lemma handle_tmpl_shift Γ Z h i T Σ :
+  wf_tmpl Γ Z T Σ ->
+  handle_tmpl (Sub.h_shift (Sub.h_shift h 1 i) (ctx_len Γ + tctx_len Z) 0) T
+  = Sub.c_shift 
+      (handle_tmpl (Sub.h_shift h (ctx_len Γ + tctx_len Z) 0) T)
+      1 (i + (ctx_len Γ + tctx_len Z)).
+Proof.
+intros wf. induction T; simpl.
++ inv wf. apply tctx_len_gets in H5 as zlen.
+  destruct (i + (ctx_len Γ + tctx_len Z) <=? num) eqn:cmp.
+  - apply leb_complete in cmp. omega.
+  - 
+
+
+
 Fixpoint v_insert_typesafe 
   Γ v A (orig : has_vtype Γ v A) A_ins i {struct orig} :
   wf_vtype A_ins ->
@@ -24,7 +58,23 @@ with c_insert_typesafe
 with h_insert_typesafe 
   Γ h Σ D (orig : has_htype Γ h Σ D) A_ins i {struct orig} :
   wf_vtype A_ins ->
-  has_htype (ctx_insert_var Γ A_ins i) (Sub.h_shift h 1 i) Σ D.
+  has_htype (ctx_insert_var Γ A_ins i) (Sub.h_shift h 1 i) Σ D
+
+with respects_insert_typesafe
+  Γ h Σ D E (orig: respects Γ h Σ D E) A_ins i {struct orig} :
+  wf_vtype A_ins ->
+  respects (ctx_insert_var Γ A_ins i) (Sub.h_shift h 1 i) Σ D E
+
+with veq_insert_typesafe
+  Γ A v1 v2 (orig: veq A Γ v1 v2) A_ins i {struct orig} :
+  wf_vtype A_ins ->
+  veq A (ctx_insert_var Γ A_ins i) (Sub.v_shift v1 1 i) (Sub.v_shift v2 1 i)
+
+with ceq_insert_typesafe
+  Γ C c1 c2 (orig: ceq C Γ c1 c2) A_ins i {struct orig} :
+  wf_vtype A_ins ->
+  ceq C (ctx_insert_var Γ A_ins i) (Sub.c_shift c1 1 i) (Sub.c_shift c2 1 i).
+
 Proof.
 {
 intros wfins. apply TypeV.
@@ -32,10 +82,13 @@ intros wfins. apply TypeV.
 { inv orig. assumption. }
 inv orig. destruct H1.
 + clear v_insert_typesafe c_insert_typesafe h_insert_typesafe.
+  clear respects_insert_typesafe veq_insert_typesafe ceq_insert_typesafe.
   simpl. apply TypeUnit.
 + clear v_insert_typesafe c_insert_typesafe h_insert_typesafe.
+  clear respects_insert_typesafe veq_insert_typesafe ceq_insert_typesafe.
   simpl. apply TypeInt.
 + clear v_insert_typesafe c_insert_typesafe h_insert_typesafe.
+  clear respects_insert_typesafe veq_insert_typesafe ceq_insert_typesafe.
   simpl. destruct (i <=? n) eqn:cmp.
   - apply TypeVar. rewrite <-get_ctx_insert_changed.
     assumption. apply leb_complete in cmp. omega.
@@ -44,116 +97,130 @@ inv orig. destruct H1.
 + specialize (v_insert_typesafe _ _ _ H1) as IHv1.
   specialize (v_insert_typesafe _ _ _ H2) as IHv2.
   clear v_insert_typesafe c_insert_typesafe h_insert_typesafe.
-  simpl. apply TypePair. 
-  - apply IHv1; assumption.
-  - apply IHv2; assumption.
+  clear respects_insert_typesafe veq_insert_typesafe ceq_insert_typesafe.
+  simpl. apply TypePair; auto.
 + specialize (v_insert_typesafe _ _ _ H1) as IHv.
   clear v_insert_typesafe c_insert_typesafe h_insert_typesafe.
-  simpl. apply TypeInl. apply IHv; assumption.
+  clear respects_insert_typesafe veq_insert_typesafe ceq_insert_typesafe.
+  simpl. apply TypeInl. auto.
 + specialize (v_insert_typesafe _ _ _ H1) as IHv.
   clear v_insert_typesafe c_insert_typesafe h_insert_typesafe.
-  simpl. apply TypeInr. apply IHv; assumption.
+  clear respects_insert_typesafe veq_insert_typesafe ceq_insert_typesafe.
+  simpl. apply TypeInr. auto.
 + specialize (c_insert_typesafe _ _ _ H1) as IHc.
   clear v_insert_typesafe c_insert_typesafe h_insert_typesafe.
-  simpl. apply TypeFun. rewrite ctx_insert_extend.
-  apply IHc; assumption.
+  clear respects_insert_typesafe veq_insert_typesafe ceq_insert_typesafe.
+  simpl. apply TypeFun. rewrite ctx_insert_extend. auto.
 + specialize (h_insert_typesafe _ _ _ _ H2) as IHh.
   specialize (c_insert_typesafe _ _ _ H1) as IHc.
+  specialize (respects_insert_typesafe _ _ _ _ _ H3) as IHres.
   clear v_insert_typesafe c_insert_typesafe h_insert_typesafe.
-  simpl. apply TypeHandler. rewrite ctx_insert_extend. 
-  - apply IHc; assumption. 
-  - apply IHh; assumption.
+  clear respects_insert_typesafe veq_insert_typesafe ceq_insert_typesafe.
+  simpl. apply TypeHandler. rewrite ctx_insert_extend. all: auto. 
 + specialize (v_insert_typesafe _ _ _ H1) as IHv.
   clear v_insert_typesafe c_insert_typesafe h_insert_typesafe.
-  eapply TypeVSubtype. apply IHv. all: assumption.
+  clear respects_insert_typesafe veq_insert_typesafe ceq_insert_typesafe.
+  eapply TypeVSubtype; auto.
 }{
 intros wfins. apply TypeC.
-{ clear v_insert_typesafe c_insert_typesafe h_insert_typesafe.
-  apply ctx_insert_wf. inv orig. assumption. assumption. }
-{ clear v_insert_typesafe c_insert_typesafe h_insert_typesafe.
-  inv orig. assumption. }
+{ apply ctx_insert_wf. inv orig. all: assumption. }
+{ inv orig. assumption. }
 inv orig. destruct H1.
 + specialize (v_insert_typesafe _ _ _ H1) as IHv.
   clear v_insert_typesafe c_insert_typesafe h_insert_typesafe.
-  simpl. apply TypeRet. apply IHv; assumption.
+  clear respects_insert_typesafe veq_insert_typesafe ceq_insert_typesafe.
+  simpl. apply TypeRet. auto.
 + specialize (v_insert_typesafe _ _ _ H1) as IHv.
   clear v_insert_typesafe c_insert_typesafe h_insert_typesafe.
-  simpl. apply TypeAbsurd. apply IHv; assumption.
+  clear respects_insert_typesafe veq_insert_typesafe ceq_insert_typesafe.
+  simpl. apply TypeAbsurd. auto.
 + specialize (v_insert_typesafe _ _ _ H1) as IHv.
   specialize (c_insert_typesafe _ _ _ H2) as IHc.
   clear v_insert_typesafe c_insert_typesafe h_insert_typesafe.
-  eapply TypeΠMatch.
-  apply IHv. assumption.
+  clear respects_insert_typesafe veq_insert_typesafe ceq_insert_typesafe. 
+  simpl. eapply TypeΠMatch. auto.
   rewrite ctx_insert_extend. rewrite ctx_insert_extend.
-  assert (i+1+1=i+2) by omega. rewrite H3. apply IHc; assumption.
+  assert (i+1+1=i+2) by omega.  rewrite H3. auto.
 + specialize (v_insert_typesafe _ _ _ H1) as IHv.
   specialize (c_insert_typesafe _ _ _ H2) as IHc1.
   specialize (c_insert_typesafe _ _ _ H3) as IHc2.
   clear v_insert_typesafe c_insert_typesafe h_insert_typesafe.
-  simpl. eapply TypeΣMatch.
-  - apply IHv. assumption.
-  - rewrite ctx_insert_extend. apply IHc1; assumption. 
-  - rewrite ctx_insert_extend. apply IHc2; assumption. 
+  clear respects_insert_typesafe veq_insert_typesafe ceq_insert_typesafe.
+  simpl. eapply TypeΣMatch. auto. all: rewrite ctx_insert_extend; auto.
 + specialize (c_insert_typesafe _ _ _ H1) as IHc1.
   specialize (c_insert_typesafe _ _ _ H2) as IHc2.
   clear v_insert_typesafe c_insert_typesafe h_insert_typesafe.
-  simpl. eapply TypeDoBind.
-  - apply IHc1. assumption.
-  - rewrite ctx_insert_extend. apply IHc2; assumption.
+  clear respects_insert_typesafe veq_insert_typesafe ceq_insert_typesafe.
+  simpl. eapply TypeDoBind. auto. rewrite ctx_insert_extend. auto.
 + specialize (v_insert_typesafe _ _ _ H1) as IHv.
   specialize (v_insert_typesafe _ _ _ H2) as IHv0.
   clear v_insert_typesafe c_insert_typesafe h_insert_typesafe.
-  simpl. eapply TypeApp.
-  - apply IHv. assumption.
-  - apply IHv0; assumption.
+  clear respects_insert_typesafe veq_insert_typesafe ceq_insert_typesafe.
+  simpl. eapply TypeApp; auto.
 + specialize (v_insert_typesafe _ _ _ H1) as IHv.
   specialize (c_insert_typesafe _ _ _ H2) as IHc.
   clear v_insert_typesafe c_insert_typesafe h_insert_typesafe.
-  simpl. eapply TypeHandle.
-  - apply IHv. assumption.
-  - apply IHc; assumption.
+  clear respects_insert_typesafe veq_insert_typesafe ceq_insert_typesafe.
+  simpl. eapply TypeHandle; auto.
 + specialize (c_insert_typesafe _ _ _ H1) as IHc1.
   specialize (c_insert_typesafe _ _ _ H2) as IHc2.
   clear v_insert_typesafe c_insert_typesafe h_insert_typesafe.
+  clear respects_insert_typesafe veq_insert_typesafe ceq_insert_typesafe.
   simpl. eapply TypeLetRec.
-  - rewrite ctx_insert_extend. rewrite ctx_insert_extend.
-    assert (i+1+1=i+2) by omega. rewrite H3. apply IHc1. assumption.
-  - rewrite ctx_insert_extend.  apply IHc2; assumption.
+  - do 2 rewrite ctx_insert_extend.
+    assert (i+1+1=i+2) by omega. rewrite H3. auto.
+  - rewrite ctx_insert_extend. auto.
 + specialize (v_insert_typesafe _ _ _ H2) as IHv.
   specialize (c_insert_typesafe _ _ _ H3) as IHc.
   clear v_insert_typesafe c_insert_typesafe h_insert_typesafe.
-  simpl. eapply TypeOp.
-  - exact H1.
-  - apply IHv; assumption.
-  - rewrite ctx_insert_extend. apply IHc; assumption.
+  clear respects_insert_typesafe veq_insert_typesafe ceq_insert_typesafe.
+  simpl. eapply TypeOp. 3: rewrite ctx_insert_extend. all: eauto.
 + specialize (c_insert_typesafe _ _ _ H1) as IHc.
   clear v_insert_typesafe c_insert_typesafe h_insert_typesafe.
-  eapply TypeCSubtype. apply IHc. all: assumption.
+  clear respects_insert_typesafe veq_insert_typesafe ceq_insert_typesafe.
+  eapply TypeCSubtype; auto.
 }{
 intros wfins. apply TypeH.
-{ clear v_insert_typesafe c_insert_typesafe h_insert_typesafe.
-  apply ctx_insert_wf. inv orig. assumption. assumption. }
-{ clear v_insert_typesafe c_insert_typesafe h_insert_typesafe.
-  inv orig. assumption. }
-{ clear v_insert_typesafe c_insert_typesafe h_insert_typesafe.
-  inv orig. assumption. }
+{ apply ctx_insert_wf. inv orig. all: assumption. }
+{ inv orig. assumption. }
+{ inv orig. assumption. }
 inv orig. destruct H2.
 + simpl. clear v_insert_typesafe c_insert_typesafe h_insert_typesafe.
+  clear respects_insert_typesafe veq_insert_typesafe ceq_insert_typesafe.
   apply TypeCasesØ.
 + specialize (h_insert_typesafe _ _ _ _ H3) as IHh.
   specialize (c_insert_typesafe _ _ _ H4) as IHc.
   clear v_insert_typesafe c_insert_typesafe h_insert_typesafe.
+  clear respects_insert_typesafe veq_insert_typesafe ceq_insert_typesafe.
   simpl. apply TypeCasesU.
   - assert (forall h op,
-      find_op_case h op = None ->
-      find_op_case (Sub.h_shift h 1 i) op = None).
+      find_op_case h op = None -> find_op_case (Sub.h_shift h 1 i) op = None).
     * intros h' op' orig. induction h'; auto.
-      simpl in *. destruct (op'==o). discriminate.
-      apply IHh'. assumption.
-    * apply H5. assumption.
-  - apply IHh; assumption.
+      simpl in *. destruct (op'==o). discriminate. auto.
+    * auto.
+  - auto.
   - rewrite ctx_insert_extend. rewrite ctx_insert_extend.
-    assert (i+1+1=i+2) by omega. rewrite H5. apply IHc; assumption.
+    assert (i+1+1=i+2) by omega. rewrite H5. auto.
+}{
+intros wfins. apply Respects.
+{ clear v_insert_typesafe c_insert_typesafe h_insert_typesafe.
+  clear respects_insert_typesafe veq_insert_typesafe ceq_insert_typesafe.
+  apply ctx_insert_wf. inv orig. all: assumption. }
+{ inv orig. assumption. }
+{ inv orig. assumption. }
+{ inv orig. assumption. }
+inv orig. destruct H3.
++ clear v_insert_typesafe c_insert_typesafe h_insert_typesafe.
+  clear respects_insert_typesafe veq_insert_typesafe ceq_insert_typesafe.
+  apply RespectEqsØ.
++ specialize (respects_insert_typesafe _ _ _ _ _ H3) as IHres.
+  clear v_insert_typesafe c_insert_typesafe h_insert_typesafe.
+  clear respects_insert_typesafe veq_insert_typesafe ceq_insert_typesafe.
+  apply RespectEqsU. auto.
+  rewrite join_ctxs_insert_var. rewrite join_ctx_tctx_insert_var.
+  rewrite h_shift_shift.
+
+
 }
 Qed.
 
